Wychelean.lean
@@ -1,5 +1,4 @@
 import Wychelean.Hashes.SHA256
 import Wychelean.DH.X25519
 import Wychelean.Hashes.SHA3
-import Wychelean.Hashes.Keccak
 import Wychelean.Permutations.Keccak
