Wychelean/Hashes/Keccak.lean
@@ -1,2 +1,0 @@
-import Wychelean.Hashes.Keccak.Basic
-import Wychelean.Hashes.Keccak.Properties
